proof/ml-dsa-65/bindings.ec
@@ -1,0 +1,243 @@
+require import AllCore List IntDiv QFABV.
+from Jasmin require import JModel_x86.
+(* require import Array4 Array5 Array6 Array7 Array9 Array24 Array25 Array32 Array256 Array768 Array960. 
+require import WArray32 WArray512 WArray960 WArray1536. *)
+
+import BitEncoding BS2Int BitChunking.
+
+(* require import JWord_extra. *)
+
+(* ----------- BEGIN BOOL BINDINGS ---------- *)
+op bool2bits (b : bool) : bool list = [b].
+op bits2bool (b: bool list) : bool = List.nth false b 0.
+
+op i2b (i : int) = (i %% 2 <> 0).
+op b2si (b: bool) = 0.
+
+bind bitstring bool2bits bits2bool b2i b2si i2b bool 1.
+realize size_tolist by auto.
+realize tolistP by auto.
+realize oflistP by rewrite /bool2bits /bits2bool;smt(size_eq1).
+realize ofintP by rewrite /bits2bool /int2bs => i; rewrite (nth_mkseq false) //. 
+realize touintP by rewrite /bool2bits /= => bv; rewrite bs2int_cons bs2int_nil /=. 
+realize tosintP by move => bv => //. 
+
+bind op bool (/\) "and".
+realize bvandP by move=> bv1 bv2; rewrite /bool2bits /#.
+
+(* ----------- BEGIN W8 BINDINGS ---------- *)
+bind bitstring W8.w2bits W8.bits2w W8.to_uint W8.to_sint W8.of_int W8.t 8.
+realize size_tolist by auto.
+realize tolistP by auto.
+realize oflistP by smt(W8.bits2wK). 
+realize ofintP by move => *;rewrite /of_int int2bs_mod.
+realize tosintP. move => bv /=;rewrite /to_sint /smod /BVA_Top_JWord_W8_t.msb.
+have -> /=: nth false (w2bits bv) (8 - 1) = 2 ^ (8 - 1) <= to_uint bv; last by smt().
+rewrite /to_uint. 
+rewrite -{2}(cat_take_drop 7 (w2bits bv)).
+rewrite bs2int_cat size_take 1:// W8.size_w2bits /=.
+rewrite -bs2int_div 1:// /= get_to_uint /=.
+rewrite -bs2int_mod 1:// /= /to_uint.
+by smt(bs2int_range mem_range W8.size_w2bits pow2_8).
+qed.
+realize touintP by smt().
+
+
+(* -------------------------------------------------------------------- *)
+bind op [W8.t & bool] W8."_.[_]" "get".
+
+realize bvgetP by done.
+
+(* -------------------------------------------------------------------- *)
+bind op W8.t W8.andw "and".
+
+realize bvandP.
+proof.
+move=> w1 w2; apply/(eq_from_nth witness).
+- by rewrite size_map size_zip !size_w2bits.
+rewrite size_w2bits => i rg_i; rewrite (nth_map witness) /=.
+- by rewrite size_zip !size_w2bits.
+rewrite nth_zip_cond /= size_zip !size_w2bits lez_minl 1:// /=.
+rewrite 2?iftrue ~-1:/# /=.
+rewrite [nth _ (w2bits w1) _](nth_change_dfl false) ?size_w2bits 1:/#.
+rewrite [nth _ (w2bits w2) _](nth_change_dfl false) ?size_w2bits 1:/#.
+by rewrite !get_w2bits w2bitsE nth_mkseq //#.
+qed.
+
+
+
+(* ----------- BEGIN W32 BINDINGS ---------- *)
+
+bind bitstring W32.w2bits W32.bits2w W32.to_uint W32.to_sint W32.of_int W32.t 32.
+realize size_tolist by auto.
+realize tolistP by auto.
+realize oflistP by smt(W32.bits2wK). 
+realize ofintP by move => *;rewrite /of_int int2bs_mod.
+realize tosintP. move => bv /=;rewrite /to_sint /smod /BVA_Top_JWord_W32_t.msb.
+have -> /=: nth false (w2bits bv) (32 - 1) = 2 ^ (32 - 1) <= to_uint bv; last by smt().
+rewrite /to_uint. 
+rewrite -{2}(cat_take_drop 31 (w2bits bv)).
+rewrite bs2int_cat size_take 1:// W32.size_w2bits /=.
+rewrite -bs2int_div 1:// /= get_to_uint /=.
+rewrite -bs2int_mod 1:// /= /to_uint.
+by smt(bs2int_range mem_range W32.size_w2bits pow2_32).
+qed.
+realize touintP by smt().
+
+bind op W32.t W32.( + ) "add".
+realize bvaddP by exact W32.to_uintD.
+
+
+bind op W32.t W32.( * ) "mul".
+realize bvmulP by exact W32.to_uintM. 
+
+op W32_sub (a : W32.t, b: W32.t) : W32.t = 
+  a - b.
+
+bind op W32.t W32_sub "sub".
+realize bvsubP by  rewrite /W32_sub => bv1 bv2; rewrite W32.to_uintD to_uintN /= /#.
+
+bind op W32.t W32.andw "and".
+realize bvandP. 
+rewrite /andw /map2 => bv1 bv2.
+apply (eq_from_nth false);1: rewrite size_map size_zip !size_w2bits /#. 
+move => i; rewrite size_w2bits /= => ib.
+rewrite initiE 1:/# (nth_map (false,false)) /=;1: rewrite size_zip !size_w2bits /#. 
+by rewrite !nth_zip /=;1:smt(W32.size_w2bits).
+qed.
+
+bind op W32.t W32.orw "or".
+realize bvorP. 
+rewrite /orw /map2 => bv1 bv2.
+apply (eq_from_nth false);1: rewrite size_map size_zip !size_w2bits /#. 
+move => i; rewrite size_w2bits /= => ib.
+rewrite initiE 1:/# (nth_map (false,false)) /=;1: rewrite size_zip !size_w2bits /#. 
+by rewrite !nth_zip /=;1:smt(W32.size_w2bits).
+qed.
+
+op sll_32 (w1 w2 : W32.t) : W32.t =
+ if (32 <= to_uint w2)
+ then W32.zero
+ else  w1 `<<` (truncateu8 w2).
+
+bind op [W32.t] sll_32 "shl".
+realize bvshlP.
+rewrite /sll_32 => bv1 bv2.
+case : (32 <= to_uint bv2); last first.
++ rewrite /(`<<`) W32.to_uint_shl; 1: by smt(W8.to_uint_cmp).
+  rewrite /truncateu8  => bv2bnd />.
+  rewrite (pmod_small (to_uint bv2) _); smt(W32.to_uint_cmp).
+move => *. 
+have -> : to_uint bv2 = (to_uint bv2 - 32) + 32 by ring. 
+by rewrite exprD_nneg 1,2:/# /= /#.
+qed.
+
+op srl_32 (w1 w2 : W32.t) : W32.t =
+  if 32 <= (to_uint w2) then W32.zero else
+  w1 `>>` (truncateu8 w2).
+
+bind op [W32.t] srl_32 "shr".
+realize bvshrP.
+rewrite /srl_32 => bv1 bv2.
+case : (32 <= to_uint bv2); last first.
++ rewrite /(`>>`) W32.to_uint_shr; 1: by smt(W8.to_uint_cmp).
+  rewrite /truncateu8  => bv2bnd />.
+  rewrite (pmod_small (to_uint bv2) _); smt(W32.to_uint_cmp).
+move => *. 
+have -> : to_uint bv2 = (to_uint bv2 - 32) + 32 by ring. 
+rewrite exprD_nneg 1,2:/# /=. 
+smt(StdOrder.IntOrder.expr_gt0 W32.to_uint_cmp pow2_32).
+qed.
+
+op sra_32 (w1 w2 : W32.t) : W32.t =
+ W32.sar w1 (to_uint w2).
+(*
+  if (32 <= to_uint w2) then W32.zero else w1 `|>>` (truncateu8 w2).
+*)
+(* 
+bind op [W32.t] sra_32 "ashr".
+realize bvashrP.
+move => bv1 bv2; rewrite W32_sar_div; smt(W32.to_uint_cmp).
+qed.
+*)
+
+bind op [W32.t & W8.t] W4u8.truncateu8 "truncate".
+realize bvtruncateP.
+move => mv; rewrite /truncateu8 /W32.w2bits take_mkseq 1:// /= /w2bits.
+apply (eq_from_nth witness);1: by smt(size_mkseq).
+move => i; rewrite size_mkseq /= /max /= => ib.
+rewrite !nth_mkseq 1..2:// /of_int /to_uint /= get_bits2w 1:// 
+        nth_mkseq 1:// /= get_to_uint /= /to_uint /=.
+have -> /=: (0 <= i && i < 32) by smt().
+pose a := bs2int (w2bits mv). 
+rewrite {1}(divz_eq a (2^(8-i)*2^i)) !mulrA divzMDl;
+   1: by smt(StdOrder.IntOrder.expr_gt0).
+rewrite dvdz_modzDl; 1: by
+ have ->  : 2^(8-i) = 2^((8-i-1)+1); [ by smt() |
+    rewrite exprS 1:/#; smt(dvdz_mull dvdz_mulr)].  
+by have -> : (2 ^ (8 - i) * 2 ^ i) = 256; 
+  [ rewrite -StdBigop.Bigint.Num.Domain.exprD_nneg 
+     1,2:/# /= -!addrA /= | done ].
+qed.
+
+
+(* ----------- BEGIN ARRAY BINDINGS ---------- *)
+
+from CryptoSpecs require import Array256.
+bind array Array256."_.[_]" Array256."_.[_<-_]" Array256.to_list Array256.of_list Array256.t 256.
+realize tolistP by done.
+realize get_setP by smt(Array256.get_setE). 
+realize eqP by smt(Array256.tP).
+realize get_out by smt(Array256.get_out).
+
+
+op init_256_32 (f: int -> W32.t) : W32.t Array256.t = Array256.init f.
+
+bind op [W32.t & Array256.t] init_256_32 "ainit".
+realize bvainitP.
+proof.
+rewrite /init_256_32 => f.
+rewrite BVA_Top_Array256_Array256_t.tolistP.
+apply eq_in_mkseq => i i_bnd;
+smt(Array256.initE).
+qed.
+
+from JazzEC require import BArray1024.
+
+(* ----------- BEGIN BArray1024 BINDINGS ---------- *)
+
+op BArray1024_w2bits : BArray1024.t -> bool list.
+op BArray1024_bits2w : bool list -> BArray1024.t.
+op BArray1024_to_uint : BArray1024.t -> int.
+op BArray1024_to_sint : BArray1024.t -> int.
+op BArray1024_of_int : int -> BArray1024.t.
+
+bind bitstring BArray1024_w2bits BArray1024_bits2w BArray1024_to_uint BArray1024_to_sint BArray1024_of_int BArray1024.t 8192.
+realize size_tolist by admit.
+realize tolistP by admit.
+realize oflistP by admit. 
+realize ofintP by admit.
+realize tosintP by admit.
+realize touintP by admit.
+
+bind op [BArray1024.t & W32.t] BArray1024.get32d "extract".
+realize bvextractP by admit.
+
+
+(* 
+bind array BArray1024.get8 BArray1024.set8 BArray1024.to_list BArray1024.of_list BArray1024.t 1024.
+realize tolistP by done.
+realize get_setP by smt(Array256.get_setE). 
+realize eqP by smt(Array256.tP).
+realize get_out by smt(Array256.get_out).
+
+bind op [W8.t & BArray1024] init_256_32 "ainit".
+realize bvainitP.
+proof.
+rewrite /init_256_32 => f.
+rewrite BVA_Top_Array256_Array256_t.tolistP.
+apply eq_in_mkseq => i i_bnd;
+smt(Array256.initE).
+qed.
+
+*)
